started porting spfStep

untimed/SB.thy
@@ -15,6 +15,13 @@ default_sort message
 definition sbRt :: "'m SB \<rightarrow> 'm SB" where
 "sbRt \<equiv> \<Lambda> sb. ubMapStream (Rep_cfun srt) sb"
 
+definition sbHdElem :: "'m SB \<rightarrow> (channel \<rightharpoonup> 'm discr\<^sub>\<bottom>)" where
+"sbHdElem \<equiv> \<Lambda> sb. (\<lambda>c. (c \<in> ubDom\<cdot>sb) \<leadsto> (lshd\<cdot>(sb . c)))" 
+
+definition convDiscrUp :: "(channel \<rightharpoonup> 'm) \<Rightarrow> (channel \<rightharpoonup> 'm discr\<^sub>\<bottom>)" where
+"convDiscrUp sb \<equiv> (\<lambda>c. (c \<in> dom sb) \<leadsto> (Iup (Discr (sb \<rightharpoonup> c))))"
+
+
 section \<open>Lemma\<close>
 
 subsection \<open>sbRt\<close>
@@ -26,5 +33,48 @@ lemma sbrt_cont [simp]: "cont (ubMapStream (Rep_cfun srt))"
   by (simp add: sbrt_okay ubMapStream_contI2)
 
 
+
+  
+(* ----------------------------------------------------------------------- *)
+  subsection \<open>sbHdElem\<close>
+(* ----------------------------------------------------------------------- *)    
+
+lemma sbHdElem_mono: "monofun (\<lambda> sb::'a SB. (\<lambda>c. (c \<in> ubDom\<cdot>sb) \<leadsto> (lshd\<cdot>(sb . c))))"  
+proof(rule monofunI) 
+  fix x y ::"'a SB"
+  assume "x \<sqsubseteq> y"
+  then show "(\<lambda> sb::'a SB. (\<lambda>c. (c \<in> ubDom\<cdot>sb) \<leadsto> (lshd\<cdot>(sb . c)))) x \<sqsubseteq> (\<lambda> sb::'a SB. (\<lambda>c. (c \<in> ubDom\<cdot>sb) \<leadsto> (lshd\<cdot>(sb . c)))) y"
+    by (smt below_option_def fun_below_iff monofun_cfun_arg option.discI option.sel ubdom_below)
+qed  
+  
+lemma sbHdElem_cont_pre: assumes "chain Y" shows "(\<lambda>c. (c \<in> ubDom\<cdot>(\<Squnion>i. Y i))\<leadsto>lshd\<cdot>((\<Squnion>i. Y i) . c)) \<sqsubseteq> (\<Squnion>i. (\<lambda>c. (c \<in> ubDom\<cdot>(Y i))\<leadsto>lshd\<cdot>(Y i . c)))"
+proof - 
+  fix c
+  have "(\<lambda>c. (c \<in> ubDom\<cdot>(\<Squnion>i. Y i))\<leadsto>lshd\<cdot>((\<Squnion>i. Y i) . c)) c \<sqsubseteq> (\<Squnion>i. (\<lambda>c. (c \<in> ubDom\<cdot>(Y i))\<leadsto>lshd\<cdot>(Y i . c)) c)"
+  proof(cases "c \<in> ubDom\<cdot>(\<Squnion>i. Y i)")
+    case True
+    have f1: "\<And>i. ubDom\<cdot>(\<Squnion>i. Y i) =  ubDom\<cdot>(Y i)"
+      by (simp add: assms)
+    then show ?thesis 
+      apply(simp add: True)
+    proof -
+      have "Some (lshd\<cdot>(\<Squnion>n. Y n . c)) \<sqsubseteq> (\<Squnion>n. Some (lshd\<cdot>(Y n . c)))"
+        by (metis assms ch2ch_Rep_cfunL ch2ch_Rep_cfunR if_then_lub)
+      then show "Some (lshd\<cdot>(Lub Y . c)) \<sqsubseteq> (\<Squnion>n. Some (lshd\<cdot>(Y n . c)))"
+        by (simp add: assms contlub_cfun_arg)
+    qed
+  next
+    case False
+    then show ?thesis
+      using assms by auto 
+  qed  
+  then show ?thesis
+    by (smt assms cont_pref_eq1I contlub_cfun_arg contlub_lambda eq_imp_below fun_belowI if_then_lub lub_eq op_is_lub optionLub_def po_class.chain_def some_below ubdom_chain_eq2)
+qed  
+    
+lemma sbHdElem_cont: "cont (\<lambda> sb::'a SB. (\<lambda>c. (c \<in> ubDom\<cdot>sb) \<leadsto> (lshd\<cdot>(sb . c))))"  
+  apply(rule contI2)
+  apply(auto simp add: sbHdElem_mono sbHdElem_cont_pre)
+  using sbHdElem_mono sbHdElem_cont_pre by fastforce
 
 end
