untimed/SPF.thy
@@ -1,5 +1,5 @@
 theory SPF
-  imports SB "../UFun_applyIn" UB_ToDo
+  imports SB "../UFun_applyIn" UB_ToDo "../inc/CPOFix"
 begin
 default_sort message
 
@@ -7,6 +7,16 @@ type_synonym 'm SPF = "'m SB \<Rrightarrow> 'm SB"
 
 instance ubundle :: (uscl) ubcl_comp
   sorry
+
+
+subsection \<open>spfStateFix\<close>
+  
+definition spfStateLeast :: "channel set \<Rightarrow> channel set \<Rightarrow>('s1::type \<Rightarrow> 'm SPF)" where
+"spfStateLeast In Out \<equiv> (\<lambda> x. ufLeast In Out)"
+
+definition spfStateFix ::"channel set \<Rightarrow> channel set \<Rightarrow>(('s1::type \<Rightarrow>'m SPF) \<rightarrow> ('s1 \<Rightarrow>'m SPF)) \<rightarrow> ('s1 \<Rightarrow> 'm SPF)" where
+"spfStateFix In Out \<equiv> (\<Lambda> F.  if \<forall>x. (ufDom\<cdot>((F\<cdot>(spfStateLeast In Out)) x) = In \<and> ufRan\<cdot>((F\<cdot>(spfStateLeast In Out)) x) = Out) then fixg (spfStateLeast In Out) F else (spfStateLeast In Out))"  
+
 
 section \<open>Definitions with spfApplyIn\<close>
 
@@ -22,6 +32,131 @@ definition spfConc :: "'m SB \<Rightarrow> 'm SPF \<rightarrow> 'm SPF" where
 
 
 subsection \<open>more general lemma\<close>
+
+
+subsection \<open>spfStateLeast\<close>
+        
+lemma spfStateLeast_mono: "monofun (\<lambda>x. spfLeast In Out)" 
+  by (simp add: monofunI)   
+  
+lemma spfStateLeast_cont: "cont (\<lambda>x. spfLeast In Out)"
+  by simp
+
+lemma spfStateLeast_dom [simp]: "\<forall>x. ufDom\<cdot>(spfStateLeast In Out x) = In"
+  by (simp add: spfStateLeast_def)
+
+lemma spfStateLeast_ran[simp]: "\<forall>x. ufRan\<cdot>(spfStateLeast In Out x) = Out"
+  by (simp add: spfStateLeast_def)
+
+lemma spfStateLeast_apply[simp]: 
+  assumes "ubDom\<cdot>sb = In"
+  shows "spfStateLeast In Out x \<rightleftharpoons> sb = ubLeast Out"
+  by (metis assms option.sel spfStateLeast_def ubDom_ubundle_def ufLeast_def ufleast_rep_abs)
+
+lemma spfStateLeast_bottom [simp]: assumes "\<forall>x. ufDom\<cdot>(f x) = In" and " \<forall>x. ufRan\<cdot>(f x) = Out"
+  shows "(spfStateLeast In Out) \<sqsubseteq> f"
+proof -
+  have f1: "\<forall>x. (spfStateLeast In Out x) \<sqsubseteq> f x"
+    by (simp add: assms(1) assms(2) spfStateLeast_def)
+  show ?thesis
+    by(simp add: below_fun_def f1)
+qed  
+
+subsection \<open>spfStateFix\<close>  
+
+lemma spfStateFix_mono[simp]: "monofun (\<lambda> F.  if \<forall>x. (ufDom\<cdot>((F\<cdot>(spfStateLeast In Out)) x) = In \<and> ufRan\<cdot>((F\<cdot>(spfStateLeast In Out)) x) = Out) then fixg (spfStateLeast In Out) F else (spfStateLeast In Out))"
+proof(rule monofunI)
+  fix x::"('s1::type \<Rightarrow> 'm SPF) \<rightarrow> ('s1 \<Rightarrow> 'm SPF)" and y::"('s1 \<Rightarrow>'m SPF) \<rightarrow> ('s1 \<Rightarrow>'m SPF)"
+  assume a1:"x \<sqsubseteq> y"
+  show "(if \<forall>xa. ufDom\<cdot>((x\<cdot>(spfStateLeast In Out)) xa) = In \<and> ufRan\<cdot>((x\<cdot>(spfStateLeast In Out)) xa) = Out then fixg (spfStateLeast In Out) x else spfStateLeast In Out) \<sqsubseteq>
+           (if \<forall>x. ufDom\<cdot>((y\<cdot>(spfStateLeast In Out)) x) = In \<and> ufRan\<cdot>((y\<cdot>(spfStateLeast In Out)) x) = Out then fixg (spfStateLeast In Out) y else spfStateLeast In Out)"
+  proof(cases "\<forall>xa. ufDom\<cdot>((x\<cdot>(spfStateLeast In Out)) xa) = In \<and> ufRan\<cdot>((x\<cdot>(spfStateLeast In Out)) xa) = Out")
+    case True
+    then  have h1:"\<forall>xa. ufDom\<cdot>((y\<cdot>(spfStateLeast In Out)) xa) = In \<and> ufRan\<cdot>((y\<cdot>(spfStateLeast In Out)) xa) = Out"
+      by (metis (mono_tags, lifting) a1 cfun_below_iff fun_below_iff ufdom_below_eq ufran_below)
+    then have "fixg (spfStateLeast In Out) x \<sqsubseteq> fixg (spfStateLeast In Out) y"
+      by(simp add: fixg_def lub_iter_fixg_mono_req a1 True)
+    then show ?thesis
+      by (simp add: True h1)
+  next
+    case False
+    then have h2: "\<not> (\<forall>xa. ufDom\<cdot>((y\<cdot>(spfStateLeast In Out)) xa) = In \<and> ufRan\<cdot>((y\<cdot>(spfStateLeast In Out)) xa) = Out)"
+      by (metis (mono_tags, lifting) a1 cfun_below_iff fun_below_iff ufdom_below_eq ufran_below)
+    then show ?thesis
+      by (simp add: h2 False)
+  qed
+qed
+  
+lemma spfStateFix_cont[simp]: "cont (\<lambda> F.  if \<forall>x. (ufDom\<cdot>((F\<cdot>(spfStateLeast In Out)) x) = In \<and> ufRan\<cdot>((F\<cdot>(spfStateLeast In Out)) x) = Out) then fixg (spfStateLeast In Out) F else (spfStateLeast In Out))"
+proof(rule Cont.contI2,simp)
+  fix Y:: "nat \<Rightarrow> (('s1::type \<Rightarrow>'m SPF) \<rightarrow> ('s1 \<Rightarrow>'m SPF))"
+  assume a1:"chain Y"
+  assume a2:"chain (\<lambda>i. if \<forall>x. ufDom\<cdot>((Y i\<cdot>(spfStateLeast In Out)) x) = In \<and> ufRan\<cdot>((Y i\<cdot>(spfStateLeast In Out)) x) = Out then fixg (spfStateLeast In Out) (Y i)
+                    else spfStateLeast In Out)"
+  show "(if \<forall>x. ufDom\<cdot>(((\<Squnion>i. Y i)\<cdot>(spfStateLeast In Out)) x) = In \<and> ufRan\<cdot>(((\<Squnion>i. Y i)\<cdot>(spfStateLeast In Out)) x) = Out then fixg (spfStateLeast In Out) (\<Squnion>i. Y i)
+          else spfStateLeast In Out) \<sqsubseteq>
+         (\<Squnion>i. if \<forall>x. ufDom\<cdot>((Y i\<cdot>(spfStateLeast In Out)) x) = In \<and> ufRan\<cdot>((Y i\<cdot>(spfStateLeast In Out)) x) = Out then fixg (spfStateLeast In Out) (Y i) else spfStateLeast In Out)"
+  proof(cases "\<forall>x. ufDom\<cdot>(((\<Squnion>i. Y i)\<cdot>(spfStateLeast In Out)) x) = In \<and> ufRan\<cdot>(((\<Squnion>i. Y i)\<cdot>(spfStateLeast In Out)) x) = Out")
+    case True
+      have "\<forall>i. Y i \<sqsubseteq> Y (Suc i)"
+        by (simp add: a1 po_class.chainE)
+      have f0:"\<forall>x. chain (\<lambda>i. (Y i\<cdot>(spfStateLeast In Out)) x)"
+        using a1 ch2ch_Rep_cfunL ch2ch_fun by fastforce    
+      then have h1:"\<forall>x i. ufDom\<cdot>((Y i\<cdot>(spfStateLeast In Out)) x) = In \<and> ufRan\<cdot>((Y i\<cdot>(spfStateLeast In Out)) x) = Out"
+        by (smt True a1 cfun_below_iff fun_below_iff is_ub_thelub ufdom_below_eq ufran_below)
+    then show ?thesis
+      by(simp add: True h1 fixg_def chain_lub_lub_iter_fixg a1)
+  next
+    case False
+    have f0:"\<forall>x. chain (\<lambda>i. (Y i\<cdot>(spfStateLeast In Out)) x)"
+      using a1 ch2ch_Rep_cfunL ch2ch_fun by fastforce          
+    then have f1: "\<forall>x. ufDom\<cdot>((Y elem_6\<cdot>(spfStateLeast In Out)) x) = ufDom\<cdot>((\<Squnion>i. (Y i \<cdot>(spfStateLeast In Out)))x)"
+      proof -
+        have "chain (\<lambda>n. Y n\<cdot>(spfStateLeast In Out))"
+          by (metis a1 ch2ch_Rep_cfunL)
+        then show ?thesis
+          using ch2ch_fun lub_fun ufdom_lub_eq by fastforce
+      qed
+    have f2:"\<forall>x. ufRan\<cdot>((Y elem_6\<cdot>(spfStateLeast In Out)) x) = ufRan\<cdot>((\<Squnion>i. Y i\<cdot>(spfStateLeast In Out)) x)"
+      proof -
+        have "\<And>f n s. \<not> chain f \<or> ufRan\<cdot>(f n (s::'s1)::'m SPF) = ufRan\<cdot>(Lub f s)"
+          by (metis ch2ch_fun is_ub_thelub lub_fun ufran_below)
+        then show ?thesis
+          using a1 ch2ch_Rep_cfunL by blast
+      qed
+    have f3:"\<forall>i. \<not>(\<forall>x. ufDom\<cdot>((Y i\<cdot>(spfStateLeast In Out)) x) = In \<and> ufRan\<cdot>((Y i\<cdot>(spfStateLeast In Out)) x) = Out)"
+      by (smt False a1 fun_belowD is_ub_thelub monofun_cfun_fun ufdom_below_eq ufran_below)
+    have f4: "\<And>s n. ufRan\<cdot>(\<Squnion>n. (Y n\<cdot>(spfStateLeast In Out)) s) = ufRan\<cdot>((Y n\<cdot>(spfStateLeast In Out)) s)"
+      using f0 is_ub_thelub ufran_below by blast
+      have f5: "\<And>s n. ufDom\<cdot>(\<Squnion>n. (Y n\<cdot>(spfStateLeast In Out)) s) = ufDom\<cdot>((Y n\<cdot>(spfStateLeast In Out)) s)"
+        using f0 ufdom_lub_eq by fastforce
+    show ?thesis
+      by(simp add: f3 False)
+    qed 
+qed
+
+
+lemma spfStateFix_apply[simp]: assumes "\<forall>x. ufDom\<cdot>((F\<cdot>(spfStateLeast In Out)) x) = In" and "\<forall>x. ufRan\<cdot>((F\<cdot>(spfStateLeast In Out))x) = Out" shows "spfStateFix In Out\<cdot>F = fixg (spfStateLeast In Out) F"
+  by(simp add: spfStateFix_def assms)
+    
+(*least Fixpoint*)
+    
+lemma spfStateFix_fix: assumes "\<forall>x. ufDom\<cdot>((F\<cdot>(spfStateLeast In Out)) x) = In" and "\<forall>x. ufRan\<cdot>((F\<cdot>(spfStateLeast In Out))x) = Out" shows "spfStateFix In Out\<cdot>F = F\<cdot>(spfStateFix In Out\<cdot>F)"
+proof(simp add: assms,rule fixg_fix, simp add: assms)
+  show "\<forall>y. y \<sqsubseteq> spfStateLeast In Out \<longrightarrow> spfStateLeast In Out = y"
+    by (smt fun_below_iff po_eq_conv spfStateLeast_def ufLeast_bottom ufdom_below_eq ufleast_ufRan ufleast_ufdom ufran_below)
+qed
+  
+lemma spfStateFix_least_fix: assumes "\<forall>x. ufDom\<cdot>((F\<cdot>(spfStateLeast In Out)) x) = In" 
+                             and "\<forall>x. ufRan\<cdot>((F\<cdot>(spfStateLeast In Out))x) = Out" 
+                             and "F\<cdot>y = y" and "\<forall>x. ufDom\<cdot>(y x) = In" and "\<forall>x. ufRan\<cdot>(y x) = Out"
+                           shows "spfStateFix In Out\<cdot>F \<sqsubseteq> y"
+proof(simp add: assms, rule fixg_least_fix, simp_all add: assms)
+  show "\<forall>y. y \<sqsubseteq> spfStateLeast In Out \<longrightarrow> spfStateLeast In Out = y"
+    by (smt fun_below_iff po_eq_conv spfStateLeast_def ufLeast_bottom ufdom_below_eq ufleast_ufRan ufleast_ufdom ufran_below)
+qed
+
+
 
 lemma spf_eq: assumes "ufDom\<cdot>uf1 = ufDom\<cdot>uf2"
   and "\<And>ub. ubDom\<cdot>ub = ufDom\<cdot>uf1 \<Longrightarrow> uf1 \<rightleftharpoons> ub = uf2 \<rightleftharpoons> ub"
@@ -45,6 +180,8 @@ lemma spconc_step[simp]:
   assumes "ubDom\<cdot>sb = ufDom\<cdot>spf"
   shows "(spfConc sb1\<cdot>spf)\<rightleftharpoons>sb = ubConcEq sb1\<cdot>(spf\<rightleftharpoons>sb)"
   by(simp add: spfConc_def assms)
+
+
 
 
 
